\documentclass[11pt]{article}

\usepackage{latexsym}
\usepackage{amssymb}
\usepackage{amsthm}
\usepackage{enumerate}
\usepackage{amsmath}
\usepackage{cancel}
\numberwithin{equation}{section}

\setlength{\evensidemargin}{.25in}
\setlength{\oddsidemargin}{-.25in}
\setlength{\topmargin}{-.75in}
\setlength{\textwidth}{6.5in}
\setlength{\textheight}{9.5in}
\newcommand{\due}{December 14th, 2015}
\newcommand{\HWnum}{13}
\input{"C:/Users/joeor_000/Documents/Coursework/Define.tex"}

\begin{document}
\input{../title.tex}

\section{Problem \#1}
Given the monomials 
$$1,x,x^2,x^3,..,$$
we can construct four orthogonal functions in the range $-1<x<1$ by taking the inner product
of each function with the condition
$$\inprod{f_n(x)}{f_m(x)} = 0 \ \textnormal{for} \ n\ne{m}$$
the first functions we can pick as $f_0(x) = 1$ and $f_1(x) = x$ such that
\begin{align*}
\int_{-1}^{1}f_0(x)f_1(x)dx &= \int_{-1}^{1}xdx\\
&= \left.\frac{1}{2}x^2\right|_{-1}^{1}\\
&= \frac{1}{2}-\frac{1}{2} = 0
\end{align*}
Now we use a general form $f_2(x) = a+bx+cx^2$ and find $a,b,c$ by the orthogonal condition
\begin{align*}
\int_{-1}^{1}f_0(x)f_2(x)dx = 0 &= \int_{-1}^{1}a+bx+cx^2dx\\
&=\left.ax + \frac{b}{2}x^2 + \frac{c}{3}x^3\right|_{-1}^{1}\\
&=a + \frac{b}{2} + \frac{c}{3} + a - \frac{b}{2} + \frac{c}{3}\\
&\Downarrow\\
-a &= \frac{c}{3}
\end{align*}
and
\begin{align*}
\int_{-1}^{1}f_1(x)f_2(x)dx = 0 &= \int_{-1}^{1}ax+bx^2+cx^3dx\\
&=\left.\frac{a}{2}x^2 + \frac{b}{3}x^3 + \frac{c}{4}x^4\right|_{-1}^{1}\\
&\Downarrow\\
b &= 0
\end{align*}
So we pick $a=1$ which yields
$$f_2(x) = 3x^2-1$$
now we repeat for $f_3(x) = a+bx+cx^2+dx^3$ and we find
\begin{align*}
\int_{-1}^{1}f_0(x)f_3(x)dx = 0 &= \int_{-1}^{1}a+bx+cx^2+dx^3dx\\
&=\left.ax + \frac{b}{2}x^2 + \frac{c}{3}x^3+\frac{d}{4}x^4\right|_{-1}^{1}\\
&=a + \frac{b}{2} + \frac{c}{3} + \frac{d}{4} + a - \frac{b}{2} + \frac{c}{3} -\frac{d}{4}\\
&\Downarrow\\
-a &= \frac{c}{3}
\end{align*}
and
\begin{align*}
\int_{-1}^{1}f_1(x)f_3(x)dx = 0 &= \int_{-1}^{1}ax+bx^2+cx^3+dx^4dx\\
&=\left.\frac{a}{2}x^2 + \frac{b}{3}x^3 + \frac{c}{4}x^4 + \frac{d}{5}x^5\right|_{-1}^{1}\\
&= \frac{2b}{3} + \frac{2d}{5}\\
-5b &= 3d
\end{align*}
and
\begin{align*}
\int_{-1}^{1}f_2(x)f_3(x)dx = 0 &= \int_{-1}^{1}(a+bx+cx^2+dx^3)(3x^2-1)dx\\
\Downarrow\\
c &= 0
\end{align*}
So we pick $b=-3$ and we have 
$$f_3(x) = 5x^3-3x$$
we note that these polynomials are the Legendre polynomials without the normalization constant.

\pagebreak

\section{Problem \#2}
Given the differential equation
$$p(x)y'' + r(x)y' + q(x)y + \lambda\rho(x)y = 0$$
we can multiply it by a integrating factor 
$$F(x) = \exp\left[\int^{x}\frac{r(u)-p'(u)}{p(u)}\right]du$$
where we note that
\begin{align*}
\frac{d}{dx}\left(F(x)p(x)y'\right) = F(x)p(x)y'' + F(x)r(x)y'
\end{align*}
which yields
\begin{align*}
F(x)p(x)y'' + F(x)r(x)y' + F(x)q(x)y + \lambda F(x)\rho(x)y &= \frac{d}{dx}\left(F(x)p(x)\frac{dy}{dx}\right) + F(x)q(x)y + \lambda F(x)\rho(x)y 
\end{align*}
Which is is Strum-Liouville form.

\end{document}

