\documentclass[11pt]{article}

\usepackage{latexsym}
\usepackage{amssymb}
\usepackage{amsthm}
\usepackage{enumerate}
\usepackage{amsmath}
\usepackage{cancel}
\numberwithin{equation}{section}

\setlength{\evensidemargin}{.25in}
\setlength{\oddsidemargin}{-.25in}
\setlength{\topmargin}{-.75in}
\setlength{\textwidth}{6.5in}
\setlength{\textheight}{9.5in}
\newcommand{\due}{November 11th, 2015}
\newcommand{\HWnum}{9}
\input{"C:/Users/joeor_000/Documents/Coursework/Define.tex"}

\begin{document}
\input{../title.tex}

\section{Problem \#1}
For a one-dimensional harmonic oscillator of mass, $m$, and spring constant $k$ we can 
construct a Hamiltonian by finding the Lagrangian as
$$L = \frac{1}{2}m\dot{q}^2 - \frac{1}{2}m\omega^2q^2$$
where $\omega = \sqrt{k/m}$. We find the canonical momentum of the system as
$$p = \partiald{L}{\dot{q}} = m\dot{q}$$
which allows us to construct the Hamiltonian by
\begin{align*}
H = p\dot{q} - L  &= \frac{p^2}{m} - \frac{p^2}{2m} + \frac{1}{2}m\omega^2q^2\\
&= \frac{p^2}{2m} + \frac{1}{2}m\omega^2q^2\\
&= \frac{1}{2}m\left(\left(\frac{p}{m}\right)^2 + (\omega{q})^2\right)
\end{align*}
For the \emph{Canonical Transformation} of a one-dimensional harmonic oscillator given by
$$Q = C(p+im\omega{q}), \qquad P = C(p-im\omega{q})$$
We can find the constant $C$ by using the fact that the determinant of the Jacobian is unity. 
This implies that
\begin{align*}
1 &= \partiald{Q}{q}\partiald{P}{p} - \partiald{Q}{p}\partiald{P}{q}\\
&= (Cim\omega)C - C(-Cim\omega)\\
&= 2C^2im\omega\\
&\Downarrow\\
C &= \frac{1}{\sqrt{2im\omega}}
\end{align*}
So our transformations become
$$Q = \frac{1}{\sqrt{2im\omega}}(p+im\omega{q}), \qquad P = \frac{1}{\sqrt{2im\omega}}(p-im\omega{q})$$
Now we can find the generating function $F_2(q,P)$ for this transformation by noting that
$$\partiald{F_2}{q} = p, \qquad \partiald{F_2}{P} = Q$$
Where we can solve the transformations such that
$$p(q,P) = \sqrt{2im\omega}P+im\omega{q}$$
and
$$Q(q,P) = \frac{1}{\sqrt{2im\omega}}(p(q,P)+im\omega{q}) = P +\sqrt{2im\omega}{q}$$
Which allows us to find 
\begin{align*}
\partiald{F_2}{P} = Q  &= P +\sqrt{2im\omega}{q}\\
&\Downarrow\\
F_2(q,P) &= \frac{1}{2}P^2 +\sqrt{2im\omega}{q}P + f(q)
\end{align*}
Now we can find the function of $q$ by
\begin{align*}
\partiald{F_2}{q} = P  &= \sqrt{2im\omega}P + f'(q)\\
&\Downarrow\\
\sqrt{2im\omega}P+im\omega{q} &= \sqrt{2im\omega}P + f'(q)\\
&\Downarrow\\
f(q) = \frac{1}{2}im\omega{q^2}
\end{align*}
So our generator function is
$$F_2(q,P) = \frac{1}{2}P^2 +\sqrt{2im\omega}{q}P + \frac{1}{2}im\omega{q^2}$$
which allows us see that
\begin{align*}
QP &= \frac{1}{2im\omega}(p+im\omega{q})(p-im\omega{q})\\
&= -\frac{i}{2m\omega}(p^2+(m\omega{q})^2)\\
&= -\frac{i}{2}m\left(\frac{1}{\omega}\left(\frac{p}{m}\right)^2+\omega{q}^2\right)
\end{align*}
Which implies that the Hamiltonian is 
$$H = i\omega{QP}$$
so the equations of motion are given by
$$\dot{P} = -\partiald{H}{Q} = -i\omega{P},\qquad \dot{Q} = \partiald{H}{P} = i\omega{Q}$$
Which easily allows us to solve the equations of motion as
$$P(t) = Ae^{-i\omega{t}},\qquad Q(t) = Be^{i\omega{t}}$$

\pagebreak

\section{Problem \#2}
We note that the generator $F(q,Q) = F_1(q,Q)$ follows from the Legendre transform that states
$$\delta\int_{t_1}^{t_2}(p\dot{q}-H)-(P\dot{Q}-K)dt = 0$$
which implies that the difference in the integrand can only differ by a total time derivative
$$(p\dot{q}-H)-(P\dot{Q}-K) = \frac{dF}{dt}$$
which implies that 
$$dF = (K-H)dt + pdq - PdQ$$
We note that $F$ is a function of $q$ and $Q$. We can use this to find $F_3(p,Q)$ by noting
that
$$d(pq) = pdq + qdp$$
which allows us to write
\begin{align*}
dF &= (K-H)dt + pdq - PdQ\\
&\Downarrow\\
dF &= (K-H)dt + d(pq) - qdp - PdQ\\
&\Downarrow\\
d(F-pq) &= (K-H)dt - qdp - PdQ
\end{align*}
So $F_3(p,Q) = F-pq$. Next we repeat the process to find $F_4(p,P)$ by noting that
$$d(PQ) = PdQ + QdP$$
which implies
\begin{align*}
dF &= (K-H)dt + pdq - PdQ\\
&\Downarrow\\
dF &= (K-H)dt + d(pq) - qdp - (d(PQ) - QdP)\\
&\Downarrow\\
d(F+PQ-pq) &= (K-H)dt - qdp + QdP
\end{align*}
which implies that $F_4(p,P) = F+PQ-pq$.

\pagebreak

\section{Problem \#3}
\begin{enumerate}[(a)]
\item For the infinitesimal transformation with the generator given by
$$F_2(q,P) = qP + \epsilon{H(q,P)}$$
where $H$ is the Hamiltonian given by
$$H(q,p) = \frac{p^2}{2m} + V(q)$$
we can find the canonical transformations associated with $F_2(q,P)$ by 
\begin{align*}
Q = \partiald{F_2}{P} &= q + \epsilon\partiald{}{P}\left(\frac{P^2}{2m} + V(q)\right)\\
&= q + \epsilon\frac{P}{m}
\end{align*}
Then we can find $p$ and invert by
\begin{align*}
p = \partiald{F_2}{q} &= P + \epsilon\frac{dV}{dq}\\
&\Downarrow\\
P &= p - \epsilon\frac{dV}{dq}
\end{align*}
So replacing $P$ in the $Q$ term we get the canonical transformations 
\begin{align*}
P &= p - \epsilon\frac{dV}{dq}\\
Q &= q + \epsilon\frac{p}{m} - \frac{\epsilon^2}{m}\frac{dV}{dq}
\end{align*}

\item If we take $\epsilon$ to be a small time step we can see that for $q=q(t)$ and $p=p(t)$
we have the transformations
\begin{align*}
q(t+\epsilon) = Q &= q(t) + \epsilon\frac{p(t)}{m}\\
p(t+\epsilon) = P &= p(t) - \epsilon\frac{dV}{dq}
\end{align*}
If we Taylor expand $q(t+\epsilon)$ about $\epsilon$ to first order we see that
\begin{align*}
q(t+\epsilon) &= q(t) + \dot{q}\epsilon\\
p(t+\epsilon) &= p(t) + \dot{p}\epsilon
\end{align*}
We note that the velocity $\dot{q}$ is related to momentum $p$ by $\dot{q}=p/m$ which implies
that The $q$ expansion is the same as the canonical transformation. We also note that 
$\dot{p} = F = -dV/dq$ so the expansion of $p$ also is the same to first order.

\item Using the results from above we can find the transformed Hamiltonian $K(P,Q)$ by noting
\begin{align*}
H(q,p) &= \frac{p^2}{2m} + V(q)\\
&\Downarrow\\
K(Q,P) &= \frac{1}{2m}\left(P+\epsilon\frac{dV}{dQ}\right)^2 + V\left(Q-\epsilon\frac{P}{m}\right)\\
&= \frac{1}{2m}\left(P^2+2P\epsilon\frac{dV}{dQ}+\epsilon^2\left(\frac{dV}{dQ}\right)^2\right) + V(Q) - \epsilon\frac{P}{m}\frac{dV}{dQ} + \frac{1}{2}\epsilon^2\frac{p^2}{m^2}\frac{d^2V}{dQ^2}\\
&= \frac{P^2}{2m} + V(Q) + \epsilon\left(\frac{P}{m}\frac{dV}{dQ}-\frac{P}{m}\frac{dV}{dQ}\right) + \frac{\epsilon^2}{2m}\left(\left(\frac{dV}{dQ}\right)^2 + \frac{p^2}{m}\frac{d^2V}{dQ^2}\right)\\
&= \frac{P^2}{2m} + V(Q) +\frac{\epsilon^2}{2m}\left(\left(\frac{dV}{dQ}\right)^2 + \frac{p^2}{m}\frac{d^2V}{dQ^2}\right)
\end{align*}
\end{enumerate}

\pagebreak

\section{Problem \#4}
\begin{enumerate}[(a)]
\item For the generator 
$$F_3(p,Q) = -pQ + \epsilon{H(Q,p)}$$
where $H$ is the same Hamiltonian from problem 3 this allows up to find the transformations 
by
\begin{align*}
q = -\partiald{F_3}{p} &= Q - \epsilon\frac{p}{m}
\end{align*}
and 
$$P = -\partiald{F_3}{Q} = p - \epsilon\frac{dV}{dQ}$$
So solving for $Q$ we have the canonical transformations by noting that
$$\partiald{V}{q} = \partiald{V}{Q}\partiald{V}{q}$$
but as we can see $dQ/dq =1$ so
\begin{align*}
Q &= q + \epsilon\frac{p}{m}\\
P &= p - \epsilon\frac{dV}{dq}
\end{align*}
which are the same canonical transformations as problem 3.

\item For $\epsilon$ as a time step we can find the same result that
\begin{align*}
q(t+\epsilon) = Q &= q(t) + \epsilon\frac{p(t)}{m}\\
p(t+\epsilon) = P &= p(t) - \epsilon\frac{dV}{dq}
\end{align*}
This again is the same as the Taylor expansion about $\epsilon$ to first order. Where 
$\dot{p} = -dV/dq$ and $\dot{q} = p/m$.

\item We can find the transformed Hamiltonian by noting that
\begin{align*} 
p &= P + \epsilon\frac{dV}{dQ}\\
q &= Q - \epsilon\frac{P}{m} - \frac{\epsilon^2}{m}\frac{dV}{dQ}
\end{align*} 
\begin{align*}
H(q,p) &= \frac{p^2}{2m} + V(q)\\
&\Downarrow\\
K(Q,P) &= \frac{1}{2m}\left(P+\epsilon\frac{dV}{dQ}\right)^2 + V\left(Q-\epsilon\frac{P}{m} - \frac{\epsilon^2}{m}\frac{dV}{dQ}\right)\\
&= \frac{1}{2m}\left(P^2+2P\epsilon\frac{dV}{dQ}+\epsilon^2\left(\frac{dV}{dQ}\right)^2\right) + V(Q) - \epsilon\frac{P}{m}\frac{dV}{dQ} - \frac{\epsilon^2}{m}\left(\frac{dV}{dQ}\right)^2 + \frac{1}{2}\epsilon^2\frac{P^2}{m^2}\frac{d^2V}{dQ^2}\\
&= \frac{P^2}{2m} + V(Q) +\frac{\epsilon^2}{2m}\left(\frac{p^2}{m}\frac{d^2V}{dQ^2}-\left(\frac{dV}{dQ}\right)^2 \right)
\end{align*}

\item We see that the change from $F_2$ and $F_3$ we have to take a second order term in $Q$
because $q$ is generated from the generating function not $Q$. This results in a negative 
$(V')^2$ term. Therefore the difference between these Hamiltonians has to be related to the
time component of the generator function which is given by
$$\frac{dF}{dt} = \frac{\epsilon^2}{m}\left(\frac{dV}{dQ}\right)^2$$

\end{enumerate}

\pagebreak

\section{Problem \#5}
For the Kepler problem with a three dimensional Hamiltonian given by
$$H = \frac{\mathbf{p}^2}{2m} - \frac{k}{|\mathbf{r}|}.$$
Using this we can show that 
$$\mathbf{L} = \mathbf{r}\times\mathbf{p}$$
is a constant of motion by taking the Poisson bracket with $H$ and noting that the $l$ 
component of $\mathbf{L}$ is
$$\left(\frac{}{}\mathbf{r}\times\mathbf{p}\right)_{l} = \epsilon_{lmn}r_mp_n$$
\begin{align*}
\frac{d\mathbf{L}}{dt} = \{\mathbf{L},H\} &= \partiald{\mathbf{L}}{q_i}\partiald{H}{p_i} - \partiald{\mathbf{L}}{p_i}\partiald{H}{q_i}\\
&= (\epsilon_{lin}p_n)\frac{p_i}{m} - (\epsilon_{lmi}r_m)\left(-\frac{r_i}{|\mathbf{r}|^3}\right)\\
&= 0
\end{align*}
Note the above equation is equal to zero due to the permutations about the Levi-Civita 
symbol. Therefore the angular momentum is a conserved quantity as we expected. We can repeat
this process for 
$$\mathbf{A} = \frac{\mathbf{p}\times\mathbf{L}}{km} - \frac{\mathbf{r}}{|\mathbf{r}|}$$
where we note that the cross product is given by
\begin{align*}
(\mathbf{p}\times\mathbf{L})_m = \epsilon_{mni}p_nL_i &= \epsilon_{mni}\epsilon_{ijk}p_nr_jp_k \\
&= (\delta_{mj}\delta_{nk}-\delta_{mk}\delta_{nj})p_nr_jp_k\\
&= r_mp_kp_k - p_mr_jp_j
\end{align*}
This allows us to calculate the Poisson bracket by
\begin{align*}
\frac{d\mathbf{A}}{dt} = \{\mathbf{A},H\}  &= \partiald{\mathbf{A}}{q_i}\partiald{H}{p_i} - \partiald{\mathbf{A}}{p_i}\partiald{H}{q_i}\\
&= \left(\frac{p_k^2-p_mp_i}{km} - \frac{1}{|\mathbf{r}|} + \frac{r_i^2}{|\mathbf{r}|^3}\right)\frac{p_i}{m} - \left(\frac{2r_mp_i-p_ir_j-p_mr_i}{km}\right)\left(-\frac{r_i}{|\mathbf{r}|^3}\right)\\
&= \left(\frac{p_k^2-p_mp_i}{km} - \frac{1}{|\mathbf{r}|} + \frac{|\mathbf{r}|^2}{|\mathbf{r}|^3}\right)\frac{p_i}{m} - \left(\frac{2r_mp_i-2p_ir_j}{km}\right)\left(-\frac{r_i}{|\mathbf{r}|^3}\right)\\
&= \frac{p_ip_k^2-p_mp_i^2}{km^2} \\
&= 0
\end{align*}
So under a central potential the LRL-vector is conserved as we expect.

\end{document}

